copy_word spec

theories/examples/copy_word.v
@@ -1,7 +1,7 @@
 From machine_program_logic.program_logic Require Import weakestpre.
-From HypVeri.algebra Require Import base.
+From HypVeri.algebra Require Import base mem.
 From HypVeri.rules Require Import rules_base mov ldr str sub cmp bne.
-From HypVeri.examples Require Import instr.
+From HypVeri.examples Require Import instr loop_macro.
 From HypVeri Require Import proofmode.
 
 Section copy_word.
@@ -9,176 +9,126 @@ Section copy_word.
   Definition code src dst :=
     encode_instructions
     [
+      Mov R2 (inr R5); (* move the # of iterations to R2 *)
+      Mov R3 (inl I0);
+      Sub R2 R3; (* R5 - 1 = R2 (offset) *)
+      Mov R3 (inr R2); (* copy R2 to R3 *)
       Mov R0 (inl src);
-      Ldr R1 R0;
+      Add R2 R0;  (* src = src_base (R0) + offset (R2) *)
+      Ldr R1 R2;
       Mov R0 (inl dst);
-      Str R1 R0
+      Add R3 R0;  (* dst = dst_base (R0) + offset (R3) *)
+      Str R3 R1
     ].
 
   Context `{gen_VMG Σ}.
 
-  Lemma copy_word {ptx prx progpage srcpage dstpage sacc i q w w_ r0_ r1_} progaddr src dst :
-    ptx ≠ srcpage ->
-    prx ≠ dstpage ->
-    seq_in_page progaddr (length (code src dst)) progpage ->
-    not (addr_in_page src progpage) ->
-    not (addr_in_page dst progpage) ->
-    addr_in_page src srcpage ->
-    addr_in_page dst dstpage ->
-    progpage ∈ sacc ->
-    srcpage ∈ sacc ->
-    dstpage ∈ sacc ->
-    program (code src dst) progaddr
+  Lemma copy_word {ptx prx progpage: PID} {sacc: gset PID} {ws ws' : list Word}
+        {w r0_ r1_ r2_ r3_:Word} {i q}{iprx iptx: Imm}
+        (progaddr:Addr) (len noff :nat) (off:Word):
+    0 < noff ->
+    noff <= len ->
+    seq_in_page progaddr (length (code iprx iptx)) progpage ->
+    of_imm iprx = of_pid prx ->
+    of_imm iptx = of_pid ptx ->
+    {[progpage; prx; ptx]} ⊆ sacc ->
+    length ws = length ws' ->
+    length ws = len ->
+    (∀ i, i<= (len - noff) -> ws !! i = ws' !! i) ->
+    program (code iprx iptx) progaddr
     ∗ A@i :={q}[sacc]
     ∗ PC @@ i ->r progaddr
-    ∗ (src ->a w)
-    ∗ (dst ->a w_)
     ∗ (R0 @@ i ->r r0_)
     ∗ (R1 @@ i ->r r1_)
-    ∗ (TX@ i := ptx)
+    ∗ (R2 @@ i ->r r2_)
+    ∗ (R3 @@ i ->r r3_)
+    ∗ (R5 @@ i ->r off)
     ∗ (RX@ i := prx)
+    ∗ mem_region ws prx
+    ∗ (TX@ i := ptx)
+    ∗ mem_region ws' ptx
     ⊢ (PARWP ExecI @ i
           {{ (λ m, ⌜m = ExecI⌝
-          ∗ program (code src dst) progaddr
+          ∗ program (code iprx iptx) progaddr
           ∗ A@i :={q}[sacc]
-          ∗ PC @@ i ->r (progaddr ^+ (length (code src dst)))%f
-          ∗ src ->a w
-          ∗ dst ->a w
-          ∗ R0 @@ i ->r dst
-          ∗ R1 @@ i ->r w
+          ∗ PC @@ i ->r (progaddr ^+ (length (code iprx iptx)))%f
+          ∗ (∃ r0_, R0 @@ i ->r r0_)
+          ∗ (∃ r1_, R1 @@ i ->r r1_)
+          ∗ (∃ r2_, R2 @@ i ->r r2_)
+          ∗ (∃ r3_, R3 @@ i ->r r3_)
+          ∗ (R5 @@ i ->r off)
           ∗ (RX@ i := prx)
-          ∗ (TX@ i := ptx))}}%I).
+          ∗ (mem_region ws prx)
+          ∗ (TX@ i := ptx)
+          ∗ (∃ ws', mem_region ws' ptx ∗ ⌜ ∀ i, i <= (len - (noff-1)) -> ws !! i = ws' !! i ⌝))}}%I).
   Proof.
-    iIntros (Hneq Hneq' Hseqp Hnin Hnin' Hsrcp Hdstp Hprpain Hsrcpain Hdstpain) "(Hbstar & Hai & Hpc & Hsrc & Hdst & Hr0 & Hr1 & HTX & HRX)".
-    pose proof (seq_in_page_forall1 _ _ _ Hseqp) as Hseq.
-    rewrite <-parwp_sswp.
-    iDestruct "Hbstar" as "(p_start & Hbstar)". 
-    iApply ((mov_word progaddr src R0) with "[Hpc Hai Hr0 p_start]") ;iFrameAutoSolve.
-    2 : { apply Hprpain. }
-    apply Hseq.
-    set_solver.
-    iModIntro.
-    iIntros "(Hpc & Hinstr1 & Hacc & Hr0)".
-    rewrite <-parwp_sswp.
-    iDestruct "Hbstar" as "(p_start & Hbstar)".
-    iApply ((ldr (progaddr ^+ 1)%f src R1 R0) with "[Hpc Hacc Hr0 Hr1 Hsrc p_start HTX]");iFrameAutoSolve.
-    intros C.
-    apply to_pid_aligned_in_page in Hsrcp.
-    rewrite <-Hsrcp in Hneq.
-    rewrite C in Hneq.
-    apply Hneq.
-    reflexivity.
-    apply to_pid_aligned_in_page in Hsrcp.
-    subst srcpage.
-    assert (Hp : (progaddr ^+ 1)%f ∈ finz.seq progaddr (length (code src dst))).
-    set_solver.
-    specialize (Hseq _ Hp).
-    apply to_pid_aligned_in_page in Hseq.
-    rewrite Hseq.
-    set_solver.
-    iModIntro.
-    iIntros "(Hpc & Hinstr2 & Hr0 & Hsrc & Hr1 & Hacc & HTX)".
-    rewrite <-parwp_sswp.
-    iDestruct "Hbstar" as "(p_start & Hbstar)".
-    iApply ((mov_word ((progaddr ^+ 1) ^+ 1)%f dst R0) with "[Hpc Hacc Hr0 p_start]");iFrameAutoSolve.
-    apply Hseq. set_solver.
-    apply Hprpain.
-    iModIntro.
-    iIntros "(Hpc & Hinstr3 & Hacc & Hr0)".
-    rewrite <-parwp_sswp.
-    iDestruct "Hbstar" as "(p_start & Hbstar)".
-    iApply ((str (((progaddr ^+ 1) ^+ 1) ^+ 1)%f dst R1 R0) with "[Hpc Hacc Hr0 p_start Hdst Hr1 HRX]")
-           ;iFrameAutoSolve.
-    intros C.
-    rewrite C in Hneq'.
-    apply Hneq'.
-    apply to_pid_aligned_in_page in Hdstp.
-    assumption.
-    apply to_pid_aligned_in_page in Hdstp.
-    subst dstpage.
-    specialize (Hseq (((progaddr ^+ 1) ^+ 1) ^+ 1)%f).
-    pose proof (to_pid_aligned_in_page (((progaddr ^+ 1) ^+ 1) ^+ 1)%f progpage) as Hp.
-    assert (Hq : (((progaddr ^+ 1) ^+ 1) ^+ 1)%f ∈ finz.seq progaddr (length (code src dst))).
-    set_solver.
-    rewrite (Hp (Hseq Hq)).
-    set_solver.
-    iModIntro.
-    iIntros "(Hpc & Hinstr4 & Hr0 & Hdst & Hr1 & Hacc & HRX)".
-    iApply parwp_finish.
-    iFrame.
-    iSplit; auto.
-    assert ((progaddr ^+ length (code src dst))%f = ((((progaddr ^+ 1) ^+ 1) ^+ 1) ^+ 1)%f) as ->.
-    assert (Z.of_nat (length (code src dst)) = 4%Z) as ->. by compute.
-    solve_finz.
-    iFrame.
-  Qed.
+    Admitted.
 
-  Definition copy_word_loop step src dst :=
-    [
-    mov_word_I R5 step; (* remaining runs *)
-    mov_word_I R6 I0;    (* counter *)
-    mov_reg_I R7 PC;    (* program base address *)
-    mov_word_I R8 I2;
-    add_reg_I R7 R8;         (* loop base address *)    
-    (* loop body begin *)
-    (* loop may depend on step and counter
-       it should restore PC, R5, R6
-       perhaps, we could try to write a special rule for loops
-     *)
-    (* ldr data from src + counter to R1 *)
-    mov_word_I R8 src;
-    add_reg_I R8 R6;
-    ldr_I R9 R8;
-    (* str data from R1 to dst + counter *)
-    mov_word_I R8 dst;
-    add_reg_I R8 R6;
-    str_I R9 R8;
-    (* loop body end *)    
-    (* incr counter *)
-    mov_word_I R8 I1;
-    add_reg_I R6 R8;
-    (* decr remaining runs *)
-    sub_reg_I R5 R8;
-    (* conditional jump *)
-    (* might be a good idea to have a separate rule for branches *)
-    cmp_I R5 I0;
-    bne_I R7
-    ].
+  (* TODO: prove another spec that combine loop and the program above together, shouldn't be difficult *)
 
-  Lemma copy_words {ptx prx progpage srcpage dstpage sacc i q qi w w_ r0_ r1_} step src dst :
-    step < page_size ->
-    length mem = step ->
-    ptx ≠ srcpage ->
-    prx ≠ dstpage ->
-    seq_in_page (of_pid progpage) (length (program_c step src dst)) progpage ->
-    not (addr_in_page src progpage) ->
-    not (addr_in_page dst progpage) ->
-    addr_in_page src srcpage ->
-    addr_in_page dst dstpage ->
-    progpage ∈ sacc ->
-    srcpage ∈ sacc ->
-    dstpage ∈ sacc ->
-    program' (program_c step src dst) (of_pid progpage)
-    ∗ A@i :={q}[sacc]
-    ∗ PC @@ i ->r (of_pid progpage)
-    ∗ mem_region mem srcpage
-    ∗ (∃ m, mem_region m dstpage)
-    ∗ (R0 @@ i ->r r0_)
-    ∗ (R1 @@ i ->r r1_)
-    ∗ (TX@ i := ptx)
-    ∗ (<<i>>{ qi })
-    ∗ (RX@ i := prx)
-    ⊢ (PARWP ExecI @ i
-          {{ (λ m, ⌜m = ExecI⌝
-          ∗ program' (program_c step src dst) (of_pid progpage)
-          ∗ A@i :={q}[sacc]
-          ∗ PC @@ i ->r ((of_pid progpage) ^+ (length (program src dst)))%f
-          ∗ mem_region mem srcpage
-          ∗ mem_region mem dstpage
-          ∗ R0 @@ i ->r dst
-          ∗ R1 @@ i ->r w
-          ∗ (<<i>>{ qi })
-          ∗ (RX@ i := prx)
-          ∗ (TX@ i := ptx))}}%I).
-  Admitted.
-End copy_word.
+
+  (* proof of the four-instruction copy word program *)
+  (* Proof. *)
+  (*   iIntros (Hneq Hneq' Hseqp Hnin Hnin' Hsrcp Hdstp Hprpain Hsrcpain Hdstpain) "(Hbstar & Hai & Hpc & Hsrc & Hdst & Hr0 & Hr1 & HTX & HRX)". *)
+  (*   pose proof (seq_in_page_forall1 _ _ _ Hseqp) as Hseq. *)
+  (*   rewrite <-parwp_sswp. *)
+  (*   iDestruct "Hbstar" as "(p_start & Hbstar)".  *)
+  (*   iApply ((mov_word progaddr src R0) with "[Hpc Hai Hr0 p_start]") ;iFrameAutoSolve. *)
+  (*   2 : { apply Hprpain. } *)
+  (*   apply Hseq. *)
+  (*   set_solver. *)
+  (*   iModIntro. *)
+  (*   iIntros "(Hpc & Hinstr1 & Hacc & Hr0)". *)
+  (*   rewrite <-parwp_sswp. *)
+  (*   iDestruct "Hbstar" as "(p_start & Hbstar)". *)
+  (*   iApply ((ldr (progaddr ^+ 1)%f src R1 R0) with "[Hpc Hacc Hr0 Hr1 Hsrc p_start HTX]");iFrameAutoSolve. *)
+  (*   intros C. *)
+  (*   apply to_pid_aligned_in_page in Hsrcp. *)
+  (*   rewrite <-Hsrcp in Hneq. *)
+  (*   rewrite C in Hneq. *)
+  (*   apply Hneq. *)
+  (*   reflexivity. *)
+  (*   apply to_pid_aligned_in_page in Hsrcp. *)
+  (*   subst srcpage. *)
+  (*   assert (Hp : (progaddr ^+ 1)%f ∈ finz.seq progaddr (length (code src dst))). *)
+  (*   set_solver. *)
+  (*   specialize (Hseq _ Hp). *)
+  (*   apply to_pid_aligned_in_page in Hseq. *)
+  (*   rewrite Hseq. *)
+  (*   set_solver. *)
+  (*   iModIntro. *)
+  (*   iIntros "(Hpc & Hinstr2 & Hr0 & Hsrc & Hr1 & Hacc & HTX)". *)
+  (*   rewrite <-parwp_sswp. *)
+  (*   iDestruct "Hbstar" as "(p_start & Hbstar)". *)
+  (*   iApply ((mov_word ((progaddr ^+ 1) ^+ 1)%f dst R0) with "[Hpc Hacc Hr0 p_start]");iFrameAutoSolve. *)
+  (*   apply Hseq. set_solver. *)
+  (*   apply Hprpain. *)
+  (*   iModIntro. *)
+  (*   iIntros "(Hpc & Hinstr3 & Hacc & Hr0)". *)
+  (*   rewrite <-parwp_sswp. *)
+  (*   iDestruct "Hbstar" as "(p_start & Hbstar)". *)
+  (*   iApply ((str (((progaddr ^+ 1) ^+ 1) ^+ 1)%f dst R1 R0) with "[Hpc Hacc Hr0 p_start Hdst Hr1 HRX]") *)
+  (*          ;iFrameAutoSolve. *)
+  (*   intros C. *)
+  (*   rewrite C in Hneq'. *)
+  (*   apply Hneq'. *)
+  (*   apply to_pid_aligned_in_page in Hdstp. *)
+  (*   assumption. *)
+  (*   apply to_pid_aligned_in_page in Hdstp. *)
+  (*   subst dstpage. *)
+  (*   specialize (Hseq (((progaddr ^+ 1) ^+ 1) ^+ 1)%f). *)
+  (*   pose proof (to_pid_aligned_in_page (((progaddr ^+ 1) ^+ 1) ^+ 1)%f progpage) as Hp. *)
+  (*   assert (Hq : (((progaddr ^+ 1) ^+ 1) ^+ 1)%f ∈ finz.seq progaddr (length (code src dst))). *)
+  (*   set_solver. *)
+  (*   rewrite (Hp (Hseq Hq)). *)
+  (*   set_solver. *)
+  (*   iModIntro. *)
+  (*   iIntros "(Hpc & Hinstr4 & Hr0 & Hdst & Hr1 & Hacc & HRX)". *)
+  (*   iApply parwp_finish. *)
+  (*   iFrame. *)
+  (*   iSplit; auto. *)
+  (*   assert ((progaddr ^+ length (code src dst))%f = ((((progaddr ^+ 1) ^+ 1) ^+ 1) ^+ 1)%f) as ->. *)
+  (*   assert (Z.of_nat (length (code src dst)) = 4%Z) as ->. by compute. *)
+  (*   solve_finz. *)
+  (*   iFrame. *)
+  (* Qed. *)
